{
 "cells": [
  {
   "cell_type": "markdown",
   "metadata": {},
   "source": [
    "## 2\n",
    "\n",
    "### 1\n",
    "\n",
    "Magnitude:\n",
    "$\\lvert G_{ZOH}(j\\omega) \\rvert = T \\left| \\text{sinc} \\left( \\frac{\\omega T}{2} \\right) \\right| = T \\frac{\\sin\\left(\\frac{\\omega T}{2}\\right)}{\\frac{\\omega T}{2}}$\n",
    "\n",
    "$= 0.2 \\frac{\\sin\\left(10 \\times 0.2\\right)}{10 \\times 0.2 / 2}$\n",
    "\n",
    "$\\lvert G_{ZOH}(j\\omega) \\rvert = 0.1683$\n",
    "\n",
    "Phase:\n",
    "$\\angle G_{ZOH}(j\\omega) = -\\frac{\\omega T}{2} = -10 \\times \\frac{0.2}{2} = -1 \\, \\text{rad}$\n",
    "\n",
    "### 2\n",
    "\n",
    "$m\\ddot{x}(t) = f(t)$\n",
    "\n",
    "Taking Laplace:\n",
    "\n",
    "$G(s) = \\frac{X(s)}{F(s)} = \\frac{1}{ms^2}$\n",
    "\n",
    "$G(s) = \\frac{1}{s} \\cdot \\frac{1}{ms} = \\frac{1}{ms^3}$\n",
    "\n",
    "$\\therefore G(z) = \\frac{z(z+1)T}{2m(z-1)^3}$\n",
    "\n",
    "Multiplying by $(z - z^{-1})$ to get $G_{ZAS}(z)$:\n",
    "\n",
    "$G_{ZAS}(z) = (z - z^{-1}) Z \\{ G(s) \\}$\n",
    "\n",
    "$G_{ZAS}(z) = (z - z^{-1}) \\frac{z(z+1)T}{2m(z-1)^3}$\n",
    "\n",
    "Simplifying:\n",
    "\n",
    "$G_{ZAS}(z) = \\frac{(z+1)T^2}{2m(z-1)^2}$\n",
    "\n",
    "### 3\n",
    "\n",
    "**Given:**  \n",
    "$T_d = 25 \\, \\text{ms}, \\, T = 10 \\, \\text{ms}$\n",
    "\n",
    "$25 = (3 - 0.5) \\times 10$\n",
    "\n",
    "Here, $l = 3$, and $m = 0.5$.\n",
    "\n",
    "Given:\n",
    "\n",
    "$G(s) = \\frac{\\epsilon\\tau s + 1}{(\\tau s + 1)}$\n",
    "$G_s(s) = \\frac{\\epsilon\\tau s + 1}{s(\\tau s + 1)}$\n",
    "\n",
    "**Doing partial fraction:**\n",
    "\n",
    "$G(s) = \\frac{A}{s} + \\frac{B}{\\tau s + 1}$\n",
    "\n",
    "Finding $A$ and $B$:\n",
    "\n",
    "$A = 1$\n",
    "\n",
    "$B = \\tau(\\epsilon-1)$\n",
    "\n",
    "$\\therefore G(s) = \\frac{1}{s} + \\frac{\\tau(\\epsilon-1)}{\\tau s + 1}$\n",
    "\n",
    "Taking the Z-transform:\n",
    "\n",
    "$G_{ZAS}(z) = z^{-3}\\left(1 + (\\epsilon-1)\\frac{(z - 1)(e^{-5/\\tau})}{(z - e^{-T/\\tau})} \\right)$ \n",
    "\n",
    "### 4\n",
    "\n",
    "**From the figure:**\n",
    "\n",
    "$E(S) = R(S) - H(S)Y^*(S)$\n",
    "\n",
    "Again, \n",
    "\n",
    "$Y(S) = G(S)C(S)E^*(S)$\n",
    "\n",
    "$Y^*(S) = (G_C^*(S)C^*(S))E^*(S)$\n",
    "\n",
    "Now, \n",
    "\n",
    "$E^*(S) = R^*(S) - H^*(S)(GC)^*(S)E^*(S)$\n",
    "\n",
    "$\\therefore E^*(S) = \\frac{R^*(S)}{1 + ((HGC)^*)(S)}$\n",
    "\n",
    "The analog $Y(S) $ is then:\n",
    "\n",
    "$\n",
    "Y(S) = G(S)C(S)E^*(S)\n",
    "$\n",
    "\n",
    "$\n",
    "\\therefore Y(S) = G(S)C(S) \\frac{R^*(S)}{1 + (HGC)^*(S)} \\quad \\text{(ANS)}\n",
    "$\n",
    "\n",
    "Sampled $ Y^*(S) $ is the sample of $ Y(S) $. We can write:\n",
    "\n",
    "$\n",
    "Y^*(S) = (GC)^*(S)E^*(S)\n",
    "$\n",
    "\n",
    "$\n",
    "\\therefore Y^*(S) = \\frac{(GCR)^*(S)}{1 + (HGC)^*(S)} \\quad \\text{(ANS)}\n",
    "$\n",
    "\n",
    "### 5\n",
    "\n",
    "For the following system with unity feedback, find:\n",
    "\n",
    "1. The position error constant $ K_p $ (C(E) = 1).  \n",
    "2. The velocity error constant $ K_v $.  \n",
    "3. The steady-state error due to a unit step input.  \n",
    "4. The steady-state error due to a unit ramp input.\n",
    "\n",
    "The system transfer function is given as:\n",
    "\n",
    "$$\n",
    "G(z) = \\frac{0.5z + 0.2}{(z - 0.1)(z - 0.8)}\n",
    "$$\n",
    "\n",
    "From the figure, the system is **Type-0**, as it does not have any unity poles.  \n",
    "Thus, $ n = 0 $.\n",
    "\n",
    "1. Position Error Constant ($ K_p $):\n",
    "\n",
    "For a Type-0 system, $ n = 0 $, so:\n",
    "\n",
    "$$\n",
    "K_p = \\frac{N(1)}{D(1)} = \\text{constant}\n",
    "$$\n",
    "\n",
    "Substituting the values:\n",
    "\n",
    "$$\n",
    "K_p = G(1) = \\frac{0.5 \\times 1 + 0.2}{(1 - 0.1)(1 - 0.8)} = \\frac{0.7}{0.9 \\times 0.2} = 3.3333\n",
    "$$\n",
    "\n",
    "2. Steady-State Error Due to a Unit Step Input:\n",
    "\n",
    "$$\n",
    "\\text{Steady-state error} = \\frac{1}{1 + K_p}\n",
    "$$\n",
    "\n",
    "$$\n",
    "\\text{Steady-state error} = \\frac{1}{1 + 3.3333} = 0.231 \\quad \\text{(ANS)}\n",
    "$$\n",
    "\n",
    "3. Velocity Error Constant ($ K_v $):\n",
    "\n",
    "For a Type-0 system, $ n = 0 $, so:\n",
    "\n",
    "$$\n",
    "K_v = \\lim_{z \\to 1} (z - 1) \\cdot G(z) = 0\n",
    "$$\n",
    "\n",
    "$$\n",
    "\\text{So, steady-state error due to ramp input: } e(\\infty) = \\frac{1}{K_v} = \\infty\n",
    "$$\n",
    "\n",
    "4. Steady-State Error Due to a Unit Ramp Input:\n",
    "\n",
    "$$\n",
    "e(\\infty) = \\frac{1}{K_v} = \\frac{1}{0} = \\infty\n",
    "$$\n",
    "\n",
    "### 6\n",
    "\n",
    "$y(k+2) - 0.8y(k+1) + 0.07y(k) = 2u(k+1) + 0.2u(k), \\quad k = 0, 1, 2, \\dots$\n",
    "\n",
    "Step 1: Derive the Transfer Function\n",
    "Using the Z-transform of the system:\n",
    "\n",
    "$z^2 Y(z) - 0.8z Y(z) + 0.07 Y(z) = 2z U(z) + 0.2 U(z)$\n",
    "\n",
    "Simplify:\n",
    "\n",
    "$(z^2 - 0.8z + 0.07) Y(z) = (2z + 0.2) U(z)$\n",
    "\n",
    "$\\therefore G(z) = \\frac{Y(z)}{U(z)} = \\frac{2z + 0.2}{z^2 - 0.8z + 0.07}$\n",
    "\n",
    "Step 2: Check the Roots of the Denominator\n",
    "$z^2 - 0.8z + 0.07$\n",
    "\n",
    "Factoring gives:\n",
    "\n",
    "$z^2 - 0.8z + 0.07 = (z - 0.7)(z - 0.1)$\n",
    "\n",
    "The roots are$ z = 0.7$ and$ z = 0.1$.\n",
    "\n",
    "Step 3: Stability Check\n",
    "For BIBO stability, all poles of$ G(z)$ must lie inside the unit circle $|z| < 1$:\n",
    "\n",
    "* $ |0.7| < 1$\n",
    "* $ |0.1| < 1$\n",
    "\n",
    "Since both roots satisfy$ |z| < 1$, the system is **BIBO stable**.\n",
    "\n",
    "### 7\n",
    "\n",
    "Determine \n",
    "$$G_{\\text{ZAS}}(z)=\\frac{z-1}{z}\\mathcal{Z}\\left\\{\\frac{G(S)}{S}\\right\\}$$\n",
    "\n",
    "3 steps of finding $G_{\\text{ZAS}}(z)$:  \n",
    "\n",
    "Step 1: Find $\\frac{G(s)}{s}$  \n",
    "$$\\frac{G(s)}{s}=\\frac{5.8644}{s(-5.888s+1)}=\\frac{A}{s}+\\frac{B}{1-5.888s}$$\n",
    "$$5.8644=A(-5.888s+1)+Bs$$\n",
    "For $s=0$, $5.8644=A(1-0)+B\\times0\\Rightarrow A=5.8644$\n",
    "For $s=\\frac{1}{5.888}$, $5.8644=A(1-5.888\\times\\frac{1}{5.888})+B\\times\\frac{1}{5.888}\\Rightarrow B=34.52$\n",
    "$$\\frac{G(s)}{s}=\\frac{5.8644}{s(-5.888s+1)}=\\frac{5.8644}{s}+\\frac{34.52}{1-5.888s}$$\n",
    "\n",
    "Step 2: Find $\\mathcal{Z}\\left\\{\\frac{G(s)}{s}\\right\\}$\n",
    "$$\\frac{5.8644}{s}\\rightarrow5.8644\\times\\frac{z}{z-1}$$\n",
    "$$\\frac{34.52}{1-5.888s}\\Rightarrow -5.8644\\times\\frac{1}{s+\\frac{1}{-5.888}} \\rightarrow -5.8644\\times\\frac{z}{z-e^{-0.17\\times0.1}}$$\n",
    "\n",
    "$$\\mathcal{Z}\\frac{G(s)}{s}=5.8644\\times\\frac{z}{z-1}-5.8644\\times\\frac{z}{z-e^{-0.17\\times0.1}}$$\n",
    "\n",
    "Step 3: Multiply $(1-z)^{-1}$ with $\\mathcal{Z}\\left\\{\\frac{G(s)}{s}\\right\\}$\n",
    "$$G_{\\text{ZAS}}(z)=(1-z)^{-1}\\mathcal{Z}\\frac{G(s)}{s}=\\frac{z-1}{z}\\times5.8644\\times\\frac{z}{z-1}+\\frac{z-1}{z}\\times-5.8644\\times\\frac{z}{z-e^{-0.17\\times0.1}}=5.8644-5.8644\\times\\frac{z-1}{z-1.017}$$\n",
    "\n",
    "$$G_{\\text{ZAS}}(z)=5.8644-5.8644\\times\\frac{z-1}{z-1.017}=5.8644\\left(1-\\frac{z-1}{z-1.017}\\right)=\\frac{5.8644\\times-0.017}{z-1.017}=\\frac{-0.1}{z-1.017}$$\n",
    "$$C(z)=\\frac{z-1.017}{z-1}$$\n",
    "\n",
    "Due to the pole-zero cancellation on 1.017 in the loop gain, the system is not internally stable.\n",
    "\n",
    "### 8\n",
    "\n",
    "$$F(z)=z^5-0.25Z^4+0.1z^3+0.4z^2+0.3z-0.1=0$$\n",
    "\n",
    "The system order $n=5$, thus, we need to verify 6 conditions in Jury test.\n",
    "1. $F(1)\\gt0$\n",
    "2. $(-1)^5F(-1=)\\gt0$\n",
    "3. $|a_0|\\lt a_5$\n",
    "4. $|b_0|\\lt b_4$\n",
    "5. $|c_0|\\lt c_3$\n",
    "6. $|d_0|\\lt d_2$\n",
    "\n",
    "Following the steps:\n",
    "\n",
    "1. $F(1)\\gt0$\n",
    "\n",
    "$F(1) = 1 - 0.25(1) + 0.1(1) + 0.4(1) + 0.3(1) - 0.1 = 1 - 0.25 + 0.1 + 0.4 + 0.3 - 0.1 = 1.45$\n",
    "\n",
    "2. $(-1)^5F(-1=)\\gt0$\n",
    "\n",
    "$F(-1) = (-1)^5 - 0.25(-1)^4 + 0.1(-1)^3 + 0.4(-1)^2 + 0.3(-1) - 0.1 = -1 - 0.25 - 0.1 + 0.4 - 0.3 - 0.1 = -1.3$\n",
    "\n",
    "$(-1)^5 F(-1) = (-1) \\times (-1.35) = 1.35 > 0$\n",
    "\n",
    "3. $|a_0|\\lt a_5$\n",
    "\n",
    "$|a_0| = |-0.1| = 0.1 < 1 = a_5$\n",
    "\n",
    "4. $|b_0|\\lt b_4$  \n",
    "\n",
    "$F^*(z) = z^5 F\\left(\\frac{1}{z}\\right) = 1 - 0.25z + 0.1z^2 + 0.4z^3 + 0.3z^4 - 0.1z^5$\n",
    "\n",
    "$F(z) - F^*(z) = (z^5 - 0.25z^4 + 0.1z^3 + 0.4z^2 + 0.3z - 0.1) - (1 - 0.25z + 0.1z^2 + 0.4z^3 + 0.3z^4 - 0.1z^5)$\n",
    "\n",
    "$= 1.1z^5 - 0.55z^4 - 0.3z^3 + 0.3z^2 + 0.55z - 1.1$\n",
    "\n",
    "$F_1(z) = \\frac{F(z) - F^*(z)}{1 - |a_0|^2} = \\frac{1.1z^5 - 0.55z^4 - 0.3z^3 + 0.3z^2 + 0.55z - 1.1}{0.99} \\approx 1.1111z^5 - 0.5556z^4 - 0.3030z^3 + 0.3030z^2 + 0.5556z - 1.1111$\n",
    "\n",
    "$F_1(z) = 1.1111z^5 - 0.5556z^4 - 0.3030z^3 + 0.3030z^2 + 0.5556z - 1.1111$\n",
    "\n",
    "$b_5 = 1.1111, \\quad b_4 = -0.5556, \\quad b_3 = -0.3030, \\quad b_2 = 0.3030, \\quad b_1 = 0.5556, \\quad b_0 = -1.1111$\n",
    "\n",
    "$|b_0| = |-1.1111| = 1.1111 \\quad \\text{and} \\quad |b_4| = |-0.5556| = 0.5556$\n",
    "\n",
    "$1.1111 > 0.5556 \\implies |b_0| > |b_4|$\n",
    "\n",
    "5. $|c_0|\\lt c_3$\n",
    "\n",
    "$F_1^*(z) = -1.1111z^5 + 0.5556z^4 + 0.3030z^3 - 0.3030z^2 - 0.5556z + 1.1111$\n",
    "\n",
    "$F_1(z) - F_1^*(z) = 1.1111z^5 - (-1.1111z^5) + (-0.5556z^4 - 0.5556z^4) + (-0.3030z^3 - 0.3030z^3) + (0.3030z^2 + 0.3030z^2) + (0.5556z + 0.5556z) + (-1.1111 - 1.1111)$\n",
    "\n",
    "$= 2.2222z^5 - 1.1112z^4 - 0.6060z^3 + 0.6060z^2 + 1.1112z - 2.2222$\n",
    "\n",
    "$F_2(z) = \\frac{2.2222z^5 - 1.1112z^4 - 0.6060z^3 + 0.6060z^2 + 1.1112z - 2.2222}{1 - |b_0|^2} = \\frac{2.2222z^5 - 1.1112z^4 - 0.6060z^3 + 0.6060z^2 + 1.1112z - 2.2222}{1 - (1.1111)^2} = \\frac{2.2222z^5 - 1.1112z^4 - 0.6060z^3 + 0.6060z^2 + 1.1112z - 2.2222}{-0.2345}$\n",
    "\n",
    "$\\approx -9.48z^5 + 4.735z^4 + 2.583z^3 - 2.583z^2 - 4.735z + 9.48$\n",
    "\n",
    "$F_2(z) = c_5z^5 + c_4z^4 + c_3z^3 + c_2z^2 + c_1z + c_0$\n",
    "\n",
    "$\\Rightarrow c_5 = -9.48, \\quad c_4 = 4.735, \\quad c_3 = 2.583, \\quad c_2 = -2.583, \\quad c_1 = -4.735, \\quad c_0 = 9.48$\n",
    "\n",
    "$|c_0| = |9.48| = 9.48 \\quad \\text{and} \\quad |c_3| = |2.583| = 2.583$\n",
    "\n",
    "Condition 5 fails, the system is not stable.\n"
   ]
  }
 ],
 "metadata": {
  "language_info": {
   "name": "python"
  }
 },
 "nbformat": 4,
 "nbformat_minor": 2
}
